theories/Sem/Typing.v
@@ -1,0 +1,49 @@
+(*
+ * Copyright (C) BedRock Systems Inc. 2019 Gregory Malecha
+ *
+ * SPDX-License-Identifier:AGPL-3.0-or-later
+ *)
+From Cpp Require Import
+     Ast.
+
+Fixpoint type_of (e : Expr) : type :=
+  match e with
+  | Econst_ref _ t
+  | Evar _ t
+  | Echar _ t
+  | Estring _ t
+  | Eint _ t => t
+  | Ebool _ => Tbool
+  | Eunop _ _ t
+  | Ebinop _ _ _ t
+  | Ederef _ t
+  | Eaddrof _ t
+  | Eassign _ _ t
+  | Eassign_op _ _ _ t
+  | Epreinc _ t
+  | Epostinc _ t
+  | Epredec _ t
+  | Epostdec _ t
+  | Eseqand _ _ t
+  | Eseqor _ _ t
+  | Ecomma _ _ _ t
+  | Ecall _ _ t
+  | Ecast _ _ t
+  | Emember _ _ t
+  | Emember_call _ _ _ _ t
+  | Esubscript _ _ t
+  | Esize_of _ t
+  | Ealign_of _ t
+  | Econstructor _ _ t
+  | Eimplicit _ t
+  | Eif _ _ _ t
+  | Ethis t => t
+  | Enull => Tpointer Tvoid
+  (* todo(gmm): c++ seems to have a special nullptr type *)
+  | Einitlist _ t => t
+  | Enew _ _ _ t
+  | Edelete _ _ _ t
+  | Eandclean _ t
+  | Etemp _ t => t
+  | Eatomic _ _ t => t
+  end.
