theories/Sem/Wp.v
@@ -1,0 +1,261 @@
+(*
+ * Copyright (C) BedRock Systems Inc. 2019 Gregory Malecha
+ *
+ * SPDX-License-Identifier:AGPL-3.0-or-later
+ *)
+(**
+ * Definitions for the semantics
+ *
+ *)
+Require Import Coq.Classes.Morphisms.
+Require Import Coq.Lists.List.
+Require Import Coq.Strings.String.
+
+From Cpp Require Import
+     Ast.
+From Cpp.Sem Require Import
+     Util Logic Semantics.
+
+(* this applies `wp` across a list
+ *
+ * note(gmm): we consistently use this for evaluating arguments, so it should
+ * reflect parallel evaluation
+ *)
+Section wps.
+  Context {T U V : Type}.
+  Variable wp : T -> (U -> V) -> V.
+
+  Fixpoint wps (es : list T) (Q : list U -> V) : V :=
+    match es with
+    | nil => Q nil
+    | e :: es => wp e (fun v => wps es (fun vs => Q (cons v vs)))
+    end.
+End wps.
+
+
+(* Expressions *)
+Definition FreeTemps := mpred.
+
+(* `finish` denotes the sequence point for an expression *)
+Definition finish (Q : val -> mpred) (v : val) (free : FreeTemps) : mpred :=
+  free ** Q v.
+
+
+Parameter wp_lhs
+  : forall {resolve : genv},
+    thread_info -> region ->
+    Expr ->
+    (val -> FreeTemps -> mpred) -> (* result -> free -> post *)
+    mpred. (* pre-condition *)
+
+Axiom Proper_wp_lhs : forall resolve ti r e,
+    Proper ((pointwise_relation _ (pointwise_relation _ lentails)) ==> lentails)
+           (@wp_lhs resolve ti r e).
+Global Existing Instance Proper_wp_lhs.
+
+
+Parameter wp_rhs
+  : forall {resolve : genv},
+    thread_info -> region ->
+    Expr ->
+    (val -> FreeTemps -> mpred) -> (* result -> free -> post *)
+    mpred. (* pre-condition *)
+
+Axiom Proper_wp_rhs : forall resolve ti r e,
+    Proper ((pointwise_relation _ (pointwise_relation _ lentails)) ==> lentails)
+           (@wp_rhs resolve ti r e).
+Global Existing Instance Proper_wp_rhs.
+
+Section wpe.
+  Context {resolve : genv}.
+  Variable ti : thread_info.
+  Variable ρ : region.
+
+  Definition wpe (vc : ValCat)
+  : Expr -> (val -> FreeTemps -> mpred) -> mpred :=
+    match vc with
+    | Lvalue=> @wp_lhs resolve ti ρ
+    | Rvalue => @wp_rhs resolve ti ρ
+    | Xvalue => @wp_lhs resolve ti ρ
+    end.
+
+  Definition wpAny (vce : ValCat * Expr)
+  : (val -> FreeTemps -> mpred) -> mpred :=
+    let '(vc,e) := vce in
+    wpe vc e.
+
+  Definition wpAnys := fun ve Q free => wpAny ve (fun v f => Q v (f ** free)).
+End wpe.
+
+(** Statements *)
+(** continuations
+ * C++ statements can terminate in 4 ways.
+ *
+ * note(gmm): technically, they can also raise exceptions; however,
+ * our current semantics doesn't capture this. if we want to support
+ * exceptions, we should be able to add another case,
+ * `k_throw : val -> mpred`.
+ *)
+Record Kpreds :=
+  { k_normal   : mpred
+  ; k_return   : option val -> mpred
+  ; k_break    : mpred
+  ; k_continue : mpred
+  }.
+
+Definition void_return (P : mpred) : Kpreds :=
+  {| k_normal := P
+   ; k_return := fun r => match r with
+                       | None => P
+                       | Some _ => lfalse
+                       end
+   ; k_break := lfalse
+   ; k_continue := lfalse
+   |}.
+
+Definition val_return (P : val -> mpred) : Kpreds :=
+  {| k_normal := lfalse
+   ; k_return := fun r => match r with
+                       | None => lfalse
+                       | Some v => P v
+                       end
+   ; k_break := lfalse
+   ; k_continue := lfalse |}.
+
+Definition Kseq (Q : mpred) (k : Kpreds) : Kpreds :=
+  {| k_normal   := Q
+   ; k_return   := k.(k_return)
+   ; k_break    := k.(k_break)
+   ; k_continue := k.(k_continue) |}.
+
+(* loop with invariant `I` *)
+Definition Kloop (I : mpred) (Q : Kpreds) : Kpreds :=
+  {| k_break    := Q.(k_normal)
+   ; k_continue := I
+   ; k_return   := Q.(k_return)
+   ; k_normal   := Q.(k_normal) |}.
+
+Definition Kat_exit (Q : mpred -> mpred) (k : Kpreds) : Kpreds :=
+  {| k_normal   := Q k.(k_normal)
+   ; k_return v := Q (k.(k_return) v)
+   ; k_break    := Q k.(k_break)
+   ; k_continue := Q k.(k_continue) |}.
+
+Definition Kfree (a : mpred) : Kpreds -> Kpreds :=
+  Kat_exit (fun P => a ** P).
+
+
+
+Global Instance ILogicOps_Rep : ILogicOps Kpreds :=
+{ lentails P Q :=
+    P.(k_normal) |-- Q.(k_normal) /\
+    P.(k_break) |-- Q.(k_break) /\
+    P.(k_continue) |-- Q.(k_continue) /\
+    forall x, P.(k_return) x |-- Q.(k_return) x
+; ltrue :=
+    {| k_normal := ltrue
+     ; k_break := ltrue
+     ; k_continue := ltrue
+     ; k_return _ := ltrue |}
+; lfalse :=
+    {| k_normal := lfalse
+     ; k_break := lfalse
+     ; k_continue := lfalse
+     ; k_return _ := lfalse |}
+
+; land  P Q :=
+    {| k_normal   := land P.(k_normal) Q.(k_normal)
+     ; k_break    := land P.(k_break) Q.(k_break)
+     ; k_continue := land P.(k_continue) Q.(k_continue)
+     ; k_return v := land (P.(k_return) v) (Q.(k_return) v) |}
+
+; lor   P Q :=
+    {| k_normal   := lor P.(k_normal) Q.(k_normal)
+     ; k_break    := lor P.(k_break) Q.(k_break)
+     ; k_continue := lor P.(k_continue) Q.(k_continue)
+     ; k_return v := lor (P.(k_return) v) (Q.(k_return) v) |}
+
+; limpl P Q :=
+    {| k_normal   := limpl P.(k_normal) Q.(k_normal)
+     ; k_break    := limpl P.(k_break) Q.(k_break)
+     ; k_continue := limpl P.(k_continue) Q.(k_continue)
+     ; k_return v := limpl (P.(k_return) v) (Q.(k_return) v) |}
+
+; lforall T P :=
+    {| k_normal   := lforall (fun x : T => (P x).(k_normal))
+     ; k_break    := lforall (fun x : T => (P x).(k_break))
+     ; k_continue := lforall (fun x : T => (P x).(k_continue))
+     ; k_return v := lforall (fun x : T => (P x).(k_return) v) |}
+
+; lexists T P :=
+    {| k_normal   := lexists (fun x : T => (P x).(k_normal))
+     ; k_break    := lexists (fun x : T => (P x).(k_break))
+     ; k_continue := lexists (fun x : T => (P x).(k_continue))
+     ; k_return v := lexists (fun x : T => (P x).(k_return) v) |}
+}.
+Global Instance ILogic_Kpreds : ILogic Kpreds.
+Proof.
+  constructor; try red; simpl.
+  { constructor.
+    - red. firstorder.
+    - red. firstorder; etransitivity; eauto. }
+  all: try solve [ firstorder; eauto using ltrueR, lfalseL, landL1, landL2, landR, lorL , lorR1, lorR2, limplAdj, landAdj, lforallL, lforallR, lexistsL, lexistsR ].
+  { firstorder; eapply lforallR; intros; eapply H. }
+  { firstorder; eapply lexistsL; intros; eapply H. }
+Qed.
+Global Instance BILogicOps_Kpreds : BILogicOps Kpreds :=
+{ empSP      :=
+    {| k_normal   := empSP
+     ; k_break    := empSP
+     ; k_continue := empSP
+     ; k_return _ := empSP |}
+
+; sepSP  P Q :=
+    {| k_normal   := sepSP P.(k_normal) Q.(k_normal)
+     ; k_break    := sepSP P.(k_break) Q.(k_break)
+     ; k_continue := sepSP P.(k_continue) Q.(k_continue)
+     ; k_return v := sepSP (P.(k_return) v) (Q.(k_return) v) |}
+
+; wandSP P Q :=
+    {| k_normal   := wandSP P.(k_normal) Q.(k_normal)
+     ; k_break    := wandSP P.(k_break) Q.(k_break)
+     ; k_continue := wandSP P.(k_continue) Q.(k_continue)
+     ; k_return v := wandSP (P.(k_return) v) (Q.(k_return) v) |}
+
+}.
+Global Instance BILogic_Kpreds : BILogic Kpreds.
+Proof.
+  constructor; try red; simpl; eauto with typeclass_instances.
+  all: try solve [ firstorder; eauto using sepSPC1, sepSPA1, bilsep, empSPR, wandSepSPAdj ].
+  { firstorder; eapply wandSepSPAdj; eauto. }
+  { firstorder; eapply empSPR; eauto. }
+Qed.
+
+Parameter wp
+  : forall {resolve : genv}, thread_info -> region -> Ast.Stmt -> Kpreds -> mpred.
+
+Axiom Proper_wp : forall resolve ti r e,
+    Proper (lentails ==> lentails)
+           (@wp resolve ti r e).
+Global Existing Instance Proper_wp.
+
+Parameter func_ok_raw
+  : forall {resolve: genv}, thread_info -> Func -> list val -> thread_info -> (val -> mpred) -> mpred.
+
+Definition fspec {resolve} (n : val) (ls : list val) (ti : thread_info) (Q : val -> mpred) : mpred :=
+  Exists f, [| n = Vptr f |] **
+  Exists func, code_at func f ** func_ok_raw (resolve:=resolve) ti func ls ti Q.
+
+(* todo(gmm): this is because func_ok is implemented using wp. *)
+Axiom fspec_conseq:
+  forall {resolve} (p : val) (vs : list val) ti (K m : val -> mpred),
+    (forall r : val, m r |-- K r) ->
+    fspec (resolve:=resolve) p vs ti m |-- fspec (resolve:=resolve) p vs ti K.
+
+Require Import Cpp.Sem.PLogic.
+
+(* remove from the stack *)
+Definition destroy {resolve} ti (parent : Dtor_type) (cls : globname) (v : val) (Q : mpred) : mpred :=
+  Exists da, _global (dtor_name parent cls) &~ da **
+                     |> fspec (resolve:=resolve) da (v :: nil) ti
+                     (fun _ => _at (_eq v) (tany (Tref cls)) ** Q).
